Here are a few more trigonometric proofs presented in LaTeX format within square brackets:

1. **Proof of the Law of Sines**

\[
\begin{aligned}
\text{Given:} &\ \text{triangle } \triangle ABC \text{ with sides } a, b, \text{ and } c \text{ opposite angles } A, B, \text{ and } C \text{ respectively.} \\
\text{To prove:} &\ \frac{a}{\sin A} = \frac{b}{\sin B} = \frac{c}{\sin C} \\
\text{Proof:} \\
&\text{Draw the altitude from vertex } A \text{ to side } BC \text{, intersecting } BC \text{ at point } D. \\
&\text{This creates two right triangles, } \triangle ABD \text{ and } \triangle ACD. \\
&\text{In } \triangle ABD, \sin B = \frac{h}{c} \Rightarrow h = c \sin B \\
&\text{In } \triangle ACD, \sin C = \frac{h}{b} \Rightarrow h = b \sin C \\
&\text{Since both expressions equal } h, \text{ we have } c \sin B = b \sin C. \\
&\text{Dividing both sides by } \sin B \sin C \text{ gives } \frac{c}{\sin C} = \frac{b}{\sin B}. \\
&\text{Similarly, drawing the altitude from vertex } B \text{ to side } AC \text{ and from vertex } C \text{ to side } AB \text{ gives} \\
&\frac{a}{\sin A} = \frac{c}{\sin C} \text{ and } \frac{a}{\sin A} = \frac{b}{\sin B}. \\
&\text{Thus, } \frac{a}{\sin A} = \frac{b}{\sin B} = \frac{c}{\sin C}.
\end{aligned}
\]

2. **Proof of the Law of Cosines**

\[
\begin{aligned}
\text{Given:} &\ \text{triangle } \triangle ABC \text{ with sides } a, b, \text{ and } c \text{ opposite angles } A, B, \text{ and } C \text{ respectively.} \\
\text{To prove:} &\ c^2 = a^2 + b^2 - 2ab \cos C \\
\text{Proof:} \\
&\text{Draw the altitude from vertex } C \text{ to side } AB \text{, intersecting } AB \text{ at point } D. \\
&\text{This creates two right triangles, } \triangle ACD \text{ and } \triangle BCD.} \\
&\text{Let } AD = x \text{ and } DB = y. \text{ Then } x + y = a. \\
&\text{In } \triangle ACD, c^2 = h^2 + x^2 \\
&\text{In } \triangle BCD, c^2 = h^2 + y^2 \\
&\text{Also, in } \triangle ACD, \cos C = \frac{x}{b} \Rightarrow x = b \cos C \\
&\text{and in } \triangle BCD, \cos C = \frac{y}{b} \Rightarrow y = b \cos C \\
&\text{Adding the two equations for } c^2 \text{ gives} \\
&c^2 = h^2 + x^2 + h^2 + y^2 = h^2 + h^2 + x^2 + y^2 \\
&\text{But } x + y = a \text{ and } x^2 + y^2 = (x + y)^2 - 2xy = a^2 - 2xy \\
&\text{And } xy = (b \cos C)(b \cos C) = b^2 \cos^2 C \\
&\text{So } c^2 = 2h^2 + a^2 - 2b^2 \cos^2 C \\
&\text{From } \triangle ACD, h^2 = c^2 - x^2 = c^2 - b^2 \cos^2 C \\
&\text{Substituting this into the equation for } c^2 \text{ gives} \\
&c^2 = 2(c^2 - b^2 \cos^2 C) + a^2 - 2b^2 \cos^2 C \\
&c^2 = 2c^2 - 2b^2 \cos^2 C + a^2 - 2b^2 \cos^2 C \\
&c^2 = 2c^2 - 4b^2 \cos^2 C + a^2 \\
&c^2 = a^2 + b^2 - 2ab \cos C
\end{aligned}
\]

3. **Proof of the Angle Sum Identity for Sine**

\[
\begin{aligned}
\text{To prove:} &\ \sin(x + y) = \sin x \cos y + \cos x \sin y \\
\text{Proof:} \\
&\text{Consider a unit circle with point } P \text{ at angle } x \text{ and point } Q \text{ at angle } y. \\
&\text{The angle between } P \text{ and } Q \text{ is } x + y. \\
&\text{Using the distance formula, the length of the chord } PQ \text{ is} \\
&|PQ| = \sqrt{(\cos x - \cos y)^2 + (\sin x - \sin y)^2} \\
&\text{Expanding and simplifying gives} \\
&|PQ| = \sqrt{2 - 2(\cos x \cos y + \sin x \sin y)} \\
&\text{But } |PQ| \text{ can also be expressed using the sine of the angle between } P \text{ and } Q: \\
&|PQ| = 2 \sin \left( \frac{x + y}{2} \right) \\
&\text{Equating the two expressions for } |PQ| \text{ and solving for } \sin(x + y) \text{ gives} \\
&\sin(x + y) = \sin x \cos y + \cos x \sin y
\end{aligned}
\]

These proofs demonstrate some fundamental trigonometric identities and theorems, showcasing various techniques used in trigonometric proofs.