Here are several geometry proofs presented in square bracket LaTeX format:

1. **Pythagorean Theorem Proof**

\[
\begin{aligned}
&\text{Given: } \triangle ABC \text{ with } \angle C = 90^\circ \\
&\text{To Prove: } AB^2 = AC^2 + BC^2 \\
&\text{Proof: } \\
&\text{Construct a square on each side of } \triangle ABC. \\
&\text{Let the area of the square on } AB \text{ be } [AB]^2, \\
&\text{the area of the square on } AC \text{ be } [AC]^2, \\
&\text{and the area of the square on } BC \text{ be } [BC]^2. \\
&\text{Rearrange the four right triangles formed by cutting the squares on } AC \text{ and } BC \\
&\text{to form a new square with side length } AB. \\
&\text{The area of the new square is equal to the sum of the areas of the squares on } AC \text{ and } BC, \\
&\text{plus twice the area of } \triangle ABC. \\
&\text{Thus, } [AB]^2 = [AC]^2 + [BC]^2 + 2 \cdot \text{Area}(\triangle ABC). \\
&\text{Since the area of } \triangle ABC \text{ is } \frac{1}{2} \cdot AC \cdot BC, \\
&\text{we have } [AB]^2 = [AC]^2 + [BC]^2 + AC \cdot BC. \\
&\text{But the area of the new square is also equal to } [AB]^2, \\
&\text{so } [AB]^2 = [AC]^2 + [BC]^2 + AC \cdot BC - AC \cdot BC. \\
&\text{Simplifying, we get } [AB]^2 = [AC]^2 + [BC]^2. \\
&\text{Therefore, the Pythagorean Theorem is proved.}
\end{aligned}
\]

2. **Angle Sum of a Triangle**

\[
\begin{aligned}
&\text{Given: } \triangle ABC \\
&\text{To Prove: } \angle A + \angle B + \angle C = 180^\circ \\
&\text{Proof: } \\
&\text{Draw a line through point } A \text{ parallel to } BC, \text{ intersecting } AB \text{ at } D \text{ and } AC \text{ at } E. \\
&\text{Since } DE \parallel BC, \angle DAB = \angle ABC \text{ and } \angle EAC = \angle ACB \text{ (alternate interior angles)}. \\
&\text{Also, } \angle DAE = 180^\circ \text{ (straight angle)}. \\
&\text{Thus, } \angle DAB + \angle B + \angle EAC = 180^\circ. \\
&\text{Substituting the alternate interior angles, we get } \angle A + \angle B + \angle C = 180^\circ. \\
&\text{Therefore, the sum of the interior angles of a triangle is } 180^\circ.
\end{aligned}
\]

3. **Isosceles Triangle Base Angles Theorem**

\[
\begin{aligned}
&\text{Given: } \triangle ABC \text{ with } AB = AC \\
&\text{To Prove: } \angle B = \angle C \\
&\text{Proof: } \\
&\text{Construct the angle bisector of } \angle BAC, \text{ intersecting } BC \text{ at point } D. \\
&\text{Since } AB = AC, \triangle ABD \cong \triangle ACD \text{ by the SAS Congruence Postulate}. \\
&\text{(Side-Angle-Side: } AB = AC, \angle BAD = \angle CAD, AD = AD\text{)}. \\
&\text{Thus, } \angle ABD = \angle ACD \text{ (corresponding parts of congruent triangles are congruent)}. \\
&\text{But } \angle ABD = \angle B \text{ and } \angle ACD = \angle C, \\
&\text{so } \angle B = \angle C. \\
&\text{Therefore, the base angles of an isosceles triangle are congruent.}
\end{aligned}
\]

4. **Exterior Angle Theorem**

\[
\begin{aligned}
&\text{Given: } \triangle ABC \text{ with exterior angle } \angle ACD \text{ at } \angle ACB \\
&\text{To Prove: } \angle ACD = \angle BAC + \angle ABC \\
&\text{Proof: } \\
&\text{Since } \angle ACD \text{ is an exterior angle to } \triangle ABC, \\
&\text{it is equal to the sum of the two non-adjacent interior angles, } \angle BAC \text{ and } \angle ABC. \\
&\text{Thus, } \angle ACD = \angle BAC + \angle ABC. \\
&\text{Therefore, the exterior angle of a triangle is equal to the sum of the two non-adjacent interior angles.}
\end{aligned}
\]

5. **Midsegment Theorem**

\[
\begin{aligned}
&\text{Given: } \triangle ABC \text{ with midsegment } DE \text{ (where } D \text{ and } E \text{ are midpoints of } AB \text{ and } AC, \text{ respectively)} \\
&\text{To Prove: } DE \parallel BC \text{ and } DE = \frac{1}{2}BC \\
&\text{Proof: } \\
&\text{Since } D \text{ and } E \text{ are midpoints, } AD = DB \text{ and } AE = EC. \\
&\text{Construct } DF \parallel BC \text{ through } D \text{ and } EF \parallel BC \text{ through } E. \\
&\text{Since } AD = DB \text{ and } DF \parallel BC, \triangle ADF \cong \triangle DBF \text{ by the SAS Congruence Postulate}. \\
&\text{(Side-Angle-Side: } AD = DB, \angle ADF = \angle DBF = 90^\circ, DF = DF\text{)}. \\
&\text{Thus, } AF = BF. \\
&\text{Similarly, since } AE = EC \text{ and } EF \parallel BC, \triangle AEF \cong \triangle CEF \text{ by the SAS Congruence Postulate}. \\
&\text{(Side-Angle-Side: } AE = EC, \angle AEF = \angle CEF = 90^\circ, EF = EF\text{)}. \\
&\text{Thus, } AF = CF. \\
&\text{Since } AF = BF \text{ and } AF = CF, F \text{ is the midpoint of } BC. \\
&\text{Therefore, } DE \parallel BC \text{ and } DE = \frac{1}{2}BC.
\end{aligned}
\]

These proofs cover some fundamental theorems in geometry, demonstrating various techniques used in geometric proofs.